Refactor small step relations.

IL/IL.v
@@ -1,6 +1,6 @@
 Require Import List.
 Require Export Util Relations Get Drop Var Val Exp Env Map CSet AutoIndTac MoreList OptionMap.
-Require Export Events Size SmallStepCommon.
+Require Export Events Size SmallStepRelations StateType.
 Require Import SetOperations.
 
 Set Implicit Arguments.
@@ -204,7 +204,7 @@ Module F.
   Qed.
 
   Lemma step_dec
-  : reddec step.
+  : reddec2 step.
   Proof.
     hnf; intros. destruct x as [[L V] []].
     - case_eq (exp_eval V e); intros. left. do 2 eexists. eauto 20 using step.
@@ -291,7 +291,7 @@ Module I.
   Qed.
 
   Lemma step_dec
-  : reddec step.
+  : reddec2 step.
   Proof.
     hnf; intros. destruct x as [[L V] []].
     - case_eq (exp_eval V e); intros. left. do 2 eexists. eauto 20 using step.
@@ -310,3 +310,27 @@ Module I.
   Qed.
 
 End I.
+
+
+Definition state_result X (s:X*onv val*stmt) : option val :=
+  match s with
+    | (_, E, stmtReturn e) => exp_eval E e
+    | _ => None
+  end.
+
+Instance statetype_F : StateType F.state := {
+  step := F.step;
+  result := (@state_result F.labenv);
+  step_dec := F.step_dec;
+  step_internally_deterministic := F.step_internally_deterministic;
+  step_externally_determined := F.step_externally_determined
+}.
+
+
+Instance statetype_I : StateType I.state := {
+  step := I.step;
+  result := (@state_result I.labenv);
+  step_dec := I.step_dec;
+  step_internally_deterministic := I.step_internally_deterministic;
+  step_externally_determined := I.step_externally_determined
+}.
