IL/SmallStepRelations.v
@@ -1,0 +1,416 @@
+Require Import Util Get Events StateType.
+
+Set Implicit Arguments.
+
+Definition functional2 :=
+  fun (X Y : Type) (R : X -> Y -> X -> Prop)
+  => forall x (y:Y) x1 x2, R x y x1 -> R x y x2 -> x1 = x2.
+
+Lemma no_normal_step S Y R (σ σ':S) (e:Y)
+ :  normal2 R σ
+  -> R σ e σ'
+  -> False.
+Proof.
+  intros. destruct H. hnf; eauto.
+Qed.
+
+Definition activated {S} `{StateType S} (σ:S) :=
+  exists ext σ', step σ (EvtExtern ext) σ'.
+
+Lemma no_activated_tau_step {S} `{StateType S} (σ σ':S)
+ :  activated σ
+  -> step σ EvtTau σ'
+  -> False.
+Proof.
+  intros Act Step. destruct Act as [? [? Act]].
+  eapply step_internally_deterministic in Act; eauto; dcr.
+  congruence.
+Qed.
+
+Lemma activated_normal S `{StateType S} (σ:S)
+  : activated σ
+    -> normal2 step σ
+    -> False.
+Proof.
+  intros Act Norm. inv Act. firstorder.
+Qed.
+
+Arguments activated_normal [S] [H] σ _ _.
+
+
+(** ** [plus2] - transitive closure for event-labeled relations *)
+
+Inductive plus2 (X : Type) (R : X -> event -> X -> Prop)
+  : X -> list event -> X -> Prop :=
+  plus2O  x y x' el
+  : R x y x'
+    -> el = (filter_tau y nil)
+    -> plus2 R x el x'
+| plus2S x y x' yl z el
+  : R x y x'
+    -> el = (filter_tau y yl)
+    -> plus2 R x' yl z
+    -> plus2 R x el z.
+
+
+(** ** [plus2] - reflexive, transitive closure for event-labeled relations *)
+
+Inductive star2 (X : Type) (R : X -> event -> X -> Prop) : X -> list event -> X -> Prop :=
+    star2_refl : forall x : X, star2 R x nil x
+  | star2_step : forall y x x' yl z, R x y x' -> star2 R x' yl z -> star2 R x (filter_tau y yl) z.
+
+Lemma plus2_star2 X (R: X -> event -> X -> Prop) σ1 σ2 L
+  : plus2 R σ1 L σ2 -> star2 R σ1 L σ2.
+Proof.
+  intros Plus. general induction Plus; eauto using star2.
+Qed.
+
+
+Lemma star2_silent X (R:X -> event -> X -> Prop)
+  :  forall (x x' : X) (L : 〔event〕) (z : X),
+    R x EvtTau x' -> star2 R x' L z -> star2 R x L z.
+Proof.
+  intros. eapply (star2_step EvtTau); eauto.
+Qed.
+
+Lemma plus2_silent X (R:X -> event -> X -> Prop)
+  :  forall (x x' : X) (L : 〔event〕) (z : X),
+    R x EvtTau x' -> plus2 R x' L z -> plus2 R x L z.
+Proof.
+  intros. eapply (plus2S _ _ H eq_refl H0); eauto.
+Qed.
+
+Lemma star2_plus2_plus2
+     : forall (X : Type) R (x y z : X) A B,
+       star2 R x A y -> plus2 R y B z -> plus2 R x (A++B) z.
+Proof.
+  intros. general induction H; simpl; eauto using plus2.
+  - econstructor 2; eauto. rewrite filter_tau_app; eauto.
+Qed.
+
+Lemma star2_plus2_plus2_silent (X : Type) R (x y z : X) B
+  : star2 R x nil y -> plus2 R y B z -> plus2 R x B z.
+Proof.
+  intros H1 H2. eapply (star2_plus2_plus2 H1 H2).
+Qed.
+
+Lemma star2_trans
+ :  forall (X : Type) R (x y z : X) A B,
+       star2 R x A y -> star2 R y B z -> star2 R x (A++B) z.
+Proof.
+  intros. general induction H; simpl; eauto.
+  rewrite filter_tau_app.
+  eapply star2_step; eauto.
+Qed.
+
+Lemma star2_trans_silent (X : Type) R (x y z : X) B
+  : star2 R x nil y -> star2 R y B z -> star2 R x B z.
+Proof.
+  intros H1 H2. eapply (star2_trans H1 H2).
+Qed.
+
+
+Ltac relsimpl_help1 :=
+  match goal with
+  | [ H : ?R ?σ EvtTau _, H' : ?R ?σ _ _, IDet : internally_deterministic ?R
+      |- _ ] =>
+    edestruct (IDet _ _ _ _ H H');
+    clear_trivial_eqs; try clear_dup
+  | [ H : filter_tau ?y ?yl = nil |- _ ] =>
+    try (is_var y; destruct y); try (is_var yl; destruct yl);
+    invc H; simpl filter_tau in *
+  | [ H : nil = filter_tau ?y ?yl |- _ ] =>
+    try (is_var y; destruct y); try (is_var yl; destruct yl);
+    invc H; simpl filter_tau in *
+  | [ H: activated ?σ, H' : step ?σ EvtTau _ |- _ ] =>
+    exfalso; eapply (no_activated_tau_step _ H H')
+  | [ H : @step ?S ?ST ?σ EvtTau _, H' : step ?σ _ _ |- _ ] =>
+    edestruct (@step_internally_deterministic S ST _ _ _ _ H H');
+    clear_trivial_eqs; try clear_dup
+  | [ H : normal2 ?R ?σ, H' : ?R ?σ _ _ |- _ ]
+    => exfalso; eapply (no_normal_step _ _ H H')
+  | [ H : star2 _ ?σ nil ?σ |- _ ] => clear H
+  | [ H : activated ?σ, H' : normal2 _ ?σ |- _ ] =>
+    exfalso; eapply (activated_normal _ H H')
+  end.
+
+Ltac relsimpl'' :=
+    repeat relsimpl_help1.
+
+Lemma activated_star_eq S `{StateType S} (σ1 σ2:S)
+: star2 step σ1 nil σ2
+  -> activated σ1
+  -> σ1 = σ2.
+Proof.
+  intros Step1 Act. inv Step1; relsimpl''; eauto.
+Qed.
+
+Lemma normal_star_eq X (R:X -> event -> X -> Prop) (σ1 σ2:X)
+: star2 R σ1 nil σ2
+  -> normal2 R σ1
+  -> σ1 = σ2.
+Proof.
+  intros Step1 Act. inv Step1; relsimpl''; eauto.
+Qed.
+
+Lemma activated_step_reach S `{StateType S} (σ σ' σ'':S) L
+ : step σ EvtTau σ'
+   -> activated σ''
+   -> star2 step σ L σ''
+   -> star2 step σ' L σ''.
+Proof.
+  intros. inv H2; eauto; relsimpl''; eauto.
+Qed.
+
+Lemma normal_step_reach S `{StateType S} (σ σ' σ'':S) L
+ : step σ EvtTau σ'
+   -> normal2 step σ''
+   -> star2 step σ L σ''
+   -> star2 step σ' L σ''.
+Proof.
+  intros. inv H2; eauto; relsimpl''; eauto.
+Qed.
+
+Lemma inv_plus2_step X (R:X -> event -> X -> Prop) σ1 σ2 σ3 L
+  : R σ1 EvtTau σ2
+    -> internally_deterministic R
+    -> plus2 R σ1 L σ3
+    -> star2 R σ2 L σ3.
+Proof.
+  intros Single IDet Plus.
+  invc Plus.
+  - relsimpl''. simpl. econstructor.
+  - relsimpl''; simpl. eauto using plus2_star2.
+Qed.
+
+Ltac relsimpl_help2 :=
+  match goal with
+  | [ H : step ?σ EvtTau _, H' : star2 step ?σ _ ?σ', H'' : activated ?σ' |- _ ]
+    => eapply (activated_step_reach _ H H'') in H'
+  | [ H : step ?σ EvtTau _, H' : star2 step ?σ _ ?σ', H'' : normal2 _ ?σ' |- _ ]
+    => eapply (normal_step_reach _ H H'') in H'
+  | [ H : @step ?S ?ST ?σ EvtTau _,
+          H' : @plus2 ?S (@step ?S ?ST) ?σ _ _ |- _ ] =>
+    eapply (inv_plus2_step _ H (@step_internally_deterministic S ST)) in H'
+  | [ Star2 : star2 ?R ?σ _ ?σ', Norm: normal2 ?R ?σ |- _ ] =>
+    let EQ := fresh "EQ" in
+    pose proof (normal_star_eq Star2 Norm) as EQ;
+    try (is_var σ; subst σ); try (is_var σ'; subst σ')
+  | [ Star2 : star2 ?R ?σ nil ?σ', Act: activated ?σ |- _ ] =>
+    let EQ := fresh "EQ" in
+    pose proof (activated_star_eq Star2 Act) as EQ;
+    try (is_var σ; subst σ); try (is_var σ'; subst σ')
+  end.
+
+Ltac relsimpl' :=
+  repeat (first [ relsimpl_help1 | relsimpl_help2 ]).
+
+Lemma star2_reach_normal X (R:X -> event -> X -> Prop) σ1 σ2a σ2b
+: star2 R σ1 nil σ2a
+  -> normal2 R σ2a
+  -> internally_deterministic R
+  -> star2 R σ1 nil σ2b
+  -> star2 R σ2b nil σ2a.
+Proof.
+  intros Star1 Normal IDet Star2.
+  general induction Star2; relsimpl'; eauto.
+  - invc Star1; relsimpl'.
+    eauto using star2_silent.
+Qed.
+
+Lemma activated_star_reach S `{StateType S} (σ σ' σ'':S)
+: activated σ''
+  -> star2 step σ nil σ''
+  -> star2 step σ nil σ'
+  -> star2 step σ' nil σ''.
+Proof.
+  intros Act Star1 Star2. general induction Star2; relsimpl'; eauto.
+Qed.
+
+Lemma both_activated S `{StateType S} (σ1 σ2 σ3:S)
+: star2 step σ1 nil σ2
+  -> star2 step σ1 nil σ3
+  -> activated σ2
+  -> activated σ3
+  -> σ2 = σ3.
+Proof.
+  intros Step1 Step2 Act1 Act2. general induction Step2; relsimpl'; eauto.
+Qed.
+
+Lemma star2_reach_normal2 X (R:X -> event -> X -> Prop) σ1 σ2a σ2b
+: star2 R σ1 nil σ2a
+  -> star2 R σ1 nil σ2b
+  -> internally_deterministic R
+  -> normal2 R σ2a
+  -> normal2 R σ2b
+  -> σ2a = σ2b.
+Proof.
+  intros Star1 Star2 IDet Normal1 Normal2.
+  general induction Star1; relsimpl'; eauto.
+  - general induction Star2; relsimpl'; eauto.
+Qed.
+
+Ltac relsimpl_help3 :=
+  match goal with
+  | [ H : star2 ?R ?σ nil _, H' : star2 ?R ?σ _ ?σ',
+                                    H'' : activated ?σ' |- _ ]
+    => eapply (activated_star_reach H'' H') in H
+  | [ H : star2 step ?σ nil _, H' : star2 (@step ?S ?ST) ?σ _ ?σ',
+                                    H'' : normal2 _ ?σ' |- _ ]
+    => eapply (star2_reach_normal H' H'' (@step_internally_deterministic S ST)) in H
+  end.
+
+Ltac relsimpl :=
+  repeat (first [ relsimpl_help1 | relsimpl_help2 | relsimpl_help3]).
+
+Lemma activated_normal_star S `{StateType S} (σ σ' σ'':S)
+  : star2 step σ nil σ'
+    -> activated σ'
+    -> star2 step σ nil σ''
+    -> normal2 step σ''
+    -> False.
+Proof.
+  intros Star1 Act Star2 Norm; relsimpl.
+Qed.
+
+
+Ltac not_normal H :=
+  destruct H; econstructor; eexists; econstructor; eauto.
+
+
+Lemma plus2_destr_nil (X : Type) R  (x z : X)
+  : plus2 R x nil z -> exists y : X, R x EvtTau y /\ star2 R y nil z.
+Proof.
+  intros Plus. remember nil.
+  induction Plus; subst; relsimpl''; eauto using star2_refl.
+  - edestruct IHPlus; eauto; dcr.
+    eauto using star2_silent.
+Qed.
+
+Lemma star2_plus2
+: forall (X : Type) (R: X -> event -> X -> Prop) (x y z : X),
+    R x EvtTau y -> star2 R y nil z -> plus2 R x nil z.
+Proof.
+  intros. general induction H0; relsimpl'; eauto using plus2.
+  - exploit IHstar2; eauto using plus2.
+    econstructor 2; eauto; reflexivity.
+Qed.
+
+Lemma star2_reach X (R:X -> event -> X -> Prop) σ1 σ2a σ2b
+: star2 R σ1 nil σ2a
+  -> star2 R σ1 nil σ2b
+  -> internally_deterministic R
+  -> (star2 R σ2a nil σ2b \/ star2 R σ2b nil σ2a).
+Proof.
+  intros.
+  general induction H; relsimpl''; eauto using star2_silent.
+  - inv H1; relsimpl''; eauto using star2_silent.
+Qed.
+
+Inductive star2n (X : Type) (R : X -> event -> X -> Prop) : nat -> X -> list event -> X -> Prop :=
+    star2n_refl : forall x : X, star2n R 0 x nil x
+  | S_star2n n : forall y x x' yl z,
+                   R x y x'
+                   -> star2n R n x' yl z
+                   -> star2n R (S n) x (filter_tau y yl) z.
+
+Inductive plus2n (X : Type) (R : X -> event -> X -> Prop)
+: nat -> X -> list event -> X -> Prop :=
+  plus2nO x y x' el
+  : R x y x'
+    -> el = (filter_tau y nil)
+    -> plus2n R 0 x el x'
+| plus2nS n x y x' yl z el
+  : R x y x'
+    -> el = (filter_tau y yl)
+    -> plus2n R n x' yl z
+    -> plus2n R (S n)  x el z.
+
+Lemma plus2_plus2n X (R: X -> event -> X -> Prop) x A y
+: plus2 R x A y
+  -> exists n, plus2n R n x A y.
+Proof.
+  intros. general induction H.
+  - eexists; eauto using plus2n.
+  - destruct IHplus2; eexists; eauto using plus2n.
+Qed.
+
+Lemma star2n_star2 X (R: X -> event -> X -> Prop) x A y n
+: star2n R n x A y
+  -> star2 R x A y.
+Proof.
+  intros. general induction H; eauto using star2.
+Qed.
+
+Lemma plus2n_star2n X (R: X -> event -> X -> Prop) x A y n
+: plus2n R n x A y
+  -> star2n R (S n) x A y.
+Proof.
+  intros. general induction H; eauto using star2n.
+Qed.
+
+Lemma star2_star2n X (R: X -> event -> X -> Prop) x A y
+: star2 R x A y
+  -> exists n, star2n R n x A y.
+Proof.
+  intros. general induction H; eauto using star2n.
+  - destruct IHstar2; eexists; econstructor; eauto.
+Qed.
+
+Lemma star2_normal X R (x y:X)
+  : star2 R x nil y
+    -> normal2 R x
+    -> x = y.
+Proof.
+  intros. inv H; eauto.
+  exfalso. firstorder.
+Qed.
+
+Lemma star2_reach_silent_step (X : Type) (R:X -> event -> X -> Prop) (x y z : X)
+: R x EvtTau y
+  -> star2 R x nil z
+  -> internally_deterministic R
+  -> x = z \/ star2 R y nil z.
+Proof.
+  intros. inv H0; eauto.
+  exploit H1; eauto. dcr; subst; eauto.
+Qed.
+
+Ltac stuck :=
+  let A := fresh "A" in let v := fresh "v" in intros [v A]; inv A; repeat get_functional; isabsurd.
+
+Ltac stuck2 :=
+  let A := fresh "A" in
+  let v := fresh "v" in
+  let evt := fresh "evt" in
+  intros [v [evt A]]; inv A; repeat get_functional; isabsurd.
+
+
+Ltac not_activated H :=
+  let STEP := fresh "STEP" in
+  destruct H as [? [? STEP]]; inv STEP.
+
+Lemma plus2_reach X (R:X -> event -> X -> Prop) σ1 σ2a σ2b
+: plus2 R σ1 nil σ2a
+  -> plus2 R σ1 nil σ2b
+  -> internally_deterministic R
+  -> (star2 R σ2a nil σ2b \/ star2 R σ2b nil σ2a).
+Proof.
+  intros Plus1 Plus2 IDet.
+  eapply plus2_destr_nil in Plus1. eapply plus2_destr_nil in Plus2.
+  dcr. relsimpl.
+  edestruct (star2_reach H1 H3); eauto using star2_trans.
+Qed.
+
+Lemma star2n_reach X (R:X -> event -> X -> Prop) σ1 σ2a σ2b n n'
+: star2n R n σ1 nil σ2a
+  -> star2n R n' σ1 nil σ2b
+  -> internally_deterministic R
+  -> (star2n R (n'-n) σ2a nil σ2b \/ star2n R (n-n') σ2b nil σ2a).
+Proof.
+  intros Star1 Star2 IDet.
+  general induction Star1; eauto.
+  - left. orewrite (n' - 0 = n'). eauto.
+  - relsimpl. invc Star2; relsimpl; simpl; eauto.
+    right. eapply (S_star2n _ _ H Star1).
+Qed.
