TransVal/tvalTactics.v
@@ -8,7 +8,7 @@ Tactic Notation "setSubst2" hyp(A) :=
   hnf; intros; hnf in A;  eapply A; simpl; cset_tac; eauto.
 
 Tactic Notation "destructBin" hyp(A) :=
-  destruct A; try destruct A; try destruct A; try destruct A;  try destruct A; try destruct A.
+  do 6 (try destruct A).
 
 Tactic Notation "setSubstUnion" hyp(A) :=
   intros; eapply A; simpl;
